Update POET's support code to match the newer aRTA blocking bound

implementation/refinements/EDF/fast_search_space.v
@@ -13,18 +13,18 @@ Definition check_point_FP (ts : seq Task) (tsk : Task) (R : nat) (P : nat * nat)
   && (P.2 <= R).
 
 (** Further, we provide a way to compute the blocking bound when using nonpreemptive policies. *)
-Definition blocking_bound_NP (ts : seq Task) (tsk : Task) :=
-  \max_(tsk_o <- ts | (tsk_o != tsk) &&
-                     (task_deadline tsk_o > task_deadline tsk)) (task_cost tsk_o - ε).
+Definition blocking_bound_NP (ts : seq Task) (tsk : Task) (A : nat) :=
+  \max_(tsk_o <- [seq i | i <- ts] | blocking_relevant tsk_o &&
+                                   (task_deadline tsk + A <
+                                    task_deadline tsk_o)) (task_cost tsk_o - ε).
 
 (** Finally, we provide a function that checks a single point [P=(A,F)] of the search space when
     adopting a fully-nonpreemptive policy. *)
 Definition check_point_NP (ts : seq Task) (tsk : Task) (R : nat) (P : nat * nat) :=
-  (blocking_bound_NP ts tsk
+  (blocking_bound_NP ts tsk P.1
    + (task_rbf tsk (P.1 + ε) - (task_cost tsk - ε))
    + bound_on_total_hep_workload ts tsk P.1 (P.1 + P.2) <= P.1 + P.2)
   && (P.2 + (task_cost tsk - ε) <= R).
-
 
 (** * Search Space Definitions *)
 Section SearchSpaceDefinition.
